Make monotonicity into a property carried by the `iHandler` instead of achieving it by closure (and then later having to prove it anyway when writing the adequacy proof). Make less use of rewriting and equalities in favor of matching.

src/handler.v
@@ -19,23 +19,32 @@ Record iHandler Σ (EF : (Type → Type) → Type → Type) := IHandler {
     → (itree preE unit → iProp Σ)
       (* Condition [WPi Vis e k @ H; ∅ {{ Φ }}] *)
     → iProp Σ;
+    mono : ∀ preE A e Φ Φ' s s',
+        (∀ a, Φ a -∗ Φ' a) -∗
+      □ (∀ t, s t -∗ s' t) -∗
+      ihandle preE A e Φ s -∗ ihandle preE A e Φ' s';
 }.
 Arguments IHandler {_ _} _.
 
-Import EqNotations.
-(** Convenient helper for constructing [iHandler]s that treat only events with
-a particular, fixed answrer type [A]. *)
-Definition IHandlerT {Σ} {EF : (Type → Type) → Type → Type} {A : Type}
-  (H : ∀ preE, (EF preE A → (A → iProp Σ) → (itree preE unit → iProp Σ) → iProp Σ)) :
-  iHandler Σ EF :=
-  IHandler (λ preE A' e Φ s, ∃ x : A' = A, H preE
-    (rew [λ A, EF preE A] x in e)
-    (rew [λ A, (A → iProp Σ)%type] x in Φ)
-    s)%I.
+Global Instance handler_ne Σ EF n (H : iHandler Σ EF) preE A :
+  Proper ((=) ==> ((=) ==> dist n) ==> ((=) ==> dist n) ==> dist n) (ihandle _ _ H preE A).
+Proof.
+  intros e1 e2 <- Φ1 Φ2 HΦ s1 s2 Hs.
+  assert (Hmon : ∀ Φ s, (H preE A e1 Φ s ⊣⊢ ∃ Φ' s', (∀ a, Φ' a -∗ Φ a) ∗ □ (∀ a, s' a -∗ s a) ∗ H preE A e1 Φ' s')).
+  - iIntros (Φ s). iSplit.
+    * iIntros "HH". iExists Φ, s. iSplitR; first eauto. iSplitR; first eauto. done.
+    * iIntros "[%Φ' [%s' [HmonΦ [Hmons HH]]]]". iApply (mono with "[HmonΦ] [Hmons]"); eauto.
+  - rewrite !Hmon. repeat f_equiv.
+    * by apply HΦ.
+    * by apply Hs.
+Qed.
 
 (** Restricts a handler along a morphism of event types. *)
-Definition restrictH {Σ EF2} EF1 (H1 : iHandler Σ EF2) `{EF1 --< EF2} : iHandler Σ EF1 :=
-  IHandler (λ preE A e Φ s, H1 preE A (subevent A e) Φ s)%I.
+Program Definition restrictH {Σ EF2} EF1 (H1 : iHandler Σ EF2) `{EF1 --< EF2} : iHandler Σ EF1 :=
+  IHandler (λ preE A e Φ s, H1 preE A (subevent A e) Φ s)%I _.
+Next Obligation.
+  iIntros (????????????) "HΦ Hs". by iApply (mono with "[HΦ]").
+Qed.
 
 (** Asserts that the [iHandler] [H1] is stronger than [H2]. *)
 Definition subH {Σ EF} (H1 H2 : iHandler Σ EF) : iProp Σ :=
@@ -52,18 +61,3 @@ Qed.
 (** [inH H1 H2] means that, on events [E1], [H1] is stronger than [H2]. *)
 Class inH {Σ EF1 EF2} `{f : EF1 --< EF2} (H1 : iHandler Σ EF1) (H2 : iHandler Σ EF2) :=
   is_inH : ⊢ subH H1 (restrictH EF1 H2).
-
-(** Disjunction of two [iHandler]s. *)
-Global Instance iHandler_union Σ E : Union (iHandler Σ E) :=
-  λ H1 H2, IHandler (λ preE A e Φ s, H1 preE A e Φ s ∨ H2 preE A e Φ s)%I.
-
-Lemma subH_union_l Σ EF H1 H2 :
-  ⊢ subH (Σ:=Σ) (EF:=EF) H1 (H1 ∪ H2).
-Proof. iIntros (?????) "HH". by iLeft. Qed.
-Lemma subH_union_r Σ EF H1 H2 :
-  ⊢ subH (Σ:=Σ) (EF:=EF) H2 (H1 ∪ H2).
-Proof. iIntros (?????) "HH". by iRight. Qed.
-Global Instance in_union_l {Σ EF} (H1 : iHandler Σ EF) (H2 : iHandler Σ EF) : inH H1 (H1 ∪ H2).
-Proof. apply subH_union_l. Qed.
-Global Instance in_union_r {Σ E} (H1 : iHandler Σ E) (H2 : iHandler Σ E) : inH H2 (H1 ∪ H2).
-Proof. apply subH_union_r. Qed.
